Added details of instructions and memory descriptors

formalism/Assembler.v
@@ -1,2 +1,59 @@
+Require Import Omega.
 
 Inductive Register := R0 | R1 | R2 | R3 | R4 | R5 | R6 | R7 | R8 | R9 | R10 | R11.
+
+Definition Address := nat.
+Definition Value := nat.
+
+Inductive Instruction :=
+   movl : Register -> Register -> Instruction
+ | movs : Register -> Register -> Instruction
+ | movi : Register -> Value    -> Instruction
+ | add  : Register -> Register -> Instruction
+ | sub  : Register -> Register -> Instruction
+ | cmp  : Register -> Register -> Instruction
+ | jmp  : Register             -> Instruction
+ | je   : Register             -> Instruction
+ | jl   : Register             -> Instruction
+ | call : Register             -> Instruction
+ | ret  :                         Instruction
+ | halt :                         Instruction.
+
+Record MemoryDescriptor := MemDesc {
+  starting_address : nat;
+  code_size : nat;
+  data_size : nat;
+  entry_points: nat
+}.
+
+Definition last_address (m : MemoryDescriptor) : Address :=
+   starting_address m + code_size m + data_size m.
+
+
+Inductive protected : MemoryDescriptor -> Address -> Prop :=
+  Prot : forall (m : MemoryDescriptor) (p : Address), 
+    starting_address m <= p -> p < last_address m -> protected m p.
+
+Inductive unprotected : MemoryDescriptor -> Address -> Prop :=
+  Unprot_before : forall (m : MemoryDescriptor) (p : Address), 
+    p < starting_address m -> unprotected m p
+| Unprot_after :  forall (m : MemoryDescriptor) (p : Address), 
+  last_address m <= p -> unprotected m p.
+
+Lemma protected_unprotected_disjoint :
+  forall (m : MemoryDescriptor) (p : Address), not (protected m p /\ unprotected m p).
+Proof.
+  intros m p.
+  intro.
+  decompose [and] H.
+  inversion H0.
+  inversion H1 ; apply (lt_irrefl p); omega.
+Qed.
+
+
+
+
+  
+
+  
+
